WiP: adapting issue steps proof from SimTravClosure

src/travorder/TravOrderConfig.v
@@ -15,10 +15,153 @@ Require Import FairExecution.
 Require Import ImmFair.
 Require Import AuxRel2.
 Require Import TraversalOrder.
+Require Import travorder.IordTraversal.
+Require Import AuxRel2.
+(* Require Import SimTravClosure. *)
+
 
 Import ListNotations.
 
 Set Implicit Arguments.
+
+Definition iord_coherent (G: execution) (sc: relation actid) (tc: trav_label -> Prop) 
+  := dom_rel (iord G sc ;; <|tc|>) ⊆₁ tc.
+
+Record tls_coherent (G: execution) (tc: trav_label -> Prop): Prop :=
+  {
+    tls_coh_init: init_tls G ⊆₁ tc;
+    (* tls_coh_exec: tc \₁ event ↓₁ is_init ⊆₁ exec_tls G *)
+    tls_coh_exec: tc ⊆₁ init_tls G ∪₁ exec_tls G
+  }.
+
+Definition tls_coherent_alt (G: execution) (tc: trav_label -> Prop) :=
+  exists tc', tc' ⊆₁ exec_tls G /\ tc ≡₁ init_tls G ∪₁ tc'. 
+
+Lemma tls_coherent_defs_equiv (G: execution) (tc: trav_label -> Prop):
+  tls_coherent G tc <-> tls_coherent_alt G tc. 
+Proof. 
+  split; intros COH. 
+  2: { red in COH. desc. split; rewrite ?COH0, ?COH; basic_solver. }
+  destruct COH. red. exists (tc \₁ init_tls G). split.
+  { rewrite tls_coh_exec0. basic_solver. }
+  split; [| basic_solver]. 
+  rewrite (set_split_complete (init_tls G) tc) at 1. basic_solver.
+Qed.
+    
+
+Section CoherentConfigs. 
+  Variable (G: execution) (sc: relation actid). 
+  Variable (tc: trav_label -> Prop). 
+
+  (* Hypothesis (FITS: fits_graph G tc).  *)
+  (* Hypothesis (COH: iord_coherent G sc tc). *)
+  Notation "'sb'" := (sb G).
+  Notation "'rmw'" := (rmw G).
+  Notation "'data'" := (data G).
+  Notation "'addr'" := (addr G).
+  Notation "'ctrl'" := (ctrl G).
+  Notation "'rf'" := (rf G).
+  Notation "'co'" := (co G).
+  Notation "'coe'" := (coe G).
+  Notation "'fr'" := (fr G).
+
+  Notation "'fwbob'" := (fwbob G).
+  Notation "'ppo'" := (ppo G).
+  Notation "'ar'" := (ar G sc).
+  Notation "'fre'" := (fre G).
+  Notation "'rfi'" := (rfi G).
+  Notation "'rfe'" := (rfe G).
+  Notation "'deps'" := (deps G).
+  Notation "'detour'" := (detour G).
+
+  Notation "'lab'" := (lab G).
+  Notation "'loc'" := (loc lab).
+  Notation "'val'" := (val lab).
+  Notation "'mod'" := (Events.mod lab).
+  Notation "'same_loc'" := (same_loc lab).
+  
+  Notation "'E'" := (acts_set G).
+  Notation "'R'" := (fun x => is_true (is_r lab x)).
+  Notation "'W'" := (fun x => is_true (is_w lab x)).
+  Notation "'F'" := (fun x => is_true (is_f lab x)).
+  Notation "'Sc'" := (fun x => is_true (is_sc lab x)).
+  Notation "'RW'" := (R ∪₁ W).
+  Notation "'FR'" := (F ∪₁ R).
+  Notation "'FW'" := (F ∪₁ W).
+  Notation "'R_ex'" := (fun a => is_true (R_ex lab a)).
+  Notation "'W_ex'" := (W_ex G).
+  Notation "'W_ex_acq'" := (W_ex ∩₁ (fun a => is_true (is_xacq lab a))).  
+  Notation "'Rel'" := (fun x => is_true (is_rel lab x)).
+
+  Implicit Types (WF : Wf G) (COMP : complete G)
+           (WFSC : wf_sc G sc) (CONS : imm_consistent G sc)
+           (TCOH: tls_coherent G tc)
+           (ICOH: iord_coherent G sc tc).
+  
+  Lemma tlsc_I_in_W WF TCOH:
+    tc ∩₁ (action ↓₁ eq ta_issue) ⊆₁ event ↓₁ W. 
+  Proof using .
+    apply tls_coherent_defs_equiv in TCOH as [tc' [INE TC']].
+    rewrite TC', set_inter_union_l. apply set_subset_union_l. split.
+    { etransitivity; [red; intro; apply proj1| ].
+      unfold init_tls. erewrite set_pair_alt, init_w; eauto. basic_solver. }
+    rewrite INE. unfold exec_tls. rewrite !set_pair_alt.
+    unfold action, event. unfolder. ins; desf; congruence.  
+  Qed.
+  
+  Lemma tlsc_P_in_W thread WF TCOH:
+    tc ∩₁ (action ↓₁ eq (ta_propagate thread)) ⊆₁ event ↓₁ W. 
+  Proof. 
+    apply tls_coherent_defs_equiv in TCOH as [tc' [INE TC']].
+    rewrite TC', set_inter_union_l. apply set_subset_union_l. split.
+    { etransitivity; [red; intro; apply proj1| ].
+      unfold init_tls. erewrite set_pair_alt, init_w; eauto. basic_solver. }
+    rewrite INE. unfold exec_tls. rewrite !set_pair_alt.
+    unfold action, event. unfolder. ins; desf; congruence.  
+  Qed. 
+
+  Lemma exec_tls_ENI:
+    exec_tls G ⊆₁ event ↓₁ (E \₁ is_init).
+  Proof using. unfold exec_tls. rewrite !set_pair_alt. basic_solver. Qed.
+
+  Lemma init_tls_EI:
+    init_tls G ⊆₁ event ↓₁ (E ∩₁ is_init).
+  Proof using. unfold init_tls. rewrite !set_pair_alt. basic_solver. Qed.
+
+  (* Lemma tlsc_E WF TCOH: *)
+  (*   tc ⊆₁ event ↓₁ E.  *)
+  (* Proof. Admitted.  *)
+
+  Definition tlsI := tc ∩₁ (action ↓₁ eq ta_issue).
+  Definition tlsC := tc ∩₁ (action ↓₁ eq ta_cover).
+
+  
+  Lemma tlsc_w_covered_issued TCOH ICOH:
+    (* (* event ↑₁ (tc ∩₁ (action ↓₁ eq ta_cover)) ∩₁ W ⊆₁ event ↑₁ (tc ∩₁ (action ↓₁ eq ta_issue)). *) *)
+    (* ts_covered ∩₁ W ⊆₁ ts_issued. *)
+
+    (* tc ∩₁ (event ↓₁ W) ∩₁ (action ↓₁ eq ta_cover) ⊆₁ event ↓₁ (event ↑₁ (tc ∩₁ action ↓₁ eq ta_issue)). *)
+
+    tlsC ∩₁ (event ↓₁ W) ⊆₁ event ↓₁ (event ↑₁ tlsI).
+    (* (fun ae => mkTL ta_issue (event ae)) ↓₁ (tlsC ∩₁ (event ↓₁ W)) ⊆₁ tlsI. *)
+  Proof using.
+    destruct TCOH. unfold tlsC, tlsI.
+    unfolder. ins. desc. destruct x as [a e]. ins. subst.
+    
+    exists (mkTL ta_issue e). splits; eauto.
+    destruct (tls_coh_exec0 _ H) as [Il | EXl].
+    { apply tls_coh_init0. split; [basic_solver| ]. 
+      apply init_tls_EI in Il. auto. }
+    red in ICOH. apply ICOH.     
+    red. eexists. apply seq_eqv_r. split; eauto.
+    red. apply exec_tls_ENI in EXl. red. splits; try by vauto.
+    do 4 left. right. red. basic_solver 10. 
+  Qed.
+
+
+End CoherentConfigs. 
+
+
 
 Section TravOrderConfig.
   Context (G : execution) (sc : relation actid).
@@ -63,13 +206,12 @@ Notation "'R_ex'" := (fun a => is_true (R_ex lab a)).
 Notation "'W_ex'" := (W_ex G).
 Notation "'W_ex_acq'" := (W_ex ∩₁ (fun a => is_true (is_xacq lab a))).
 
-Notation "'Rel'" := (is_rel lab).
-  
-Definition iord_coherent (tc : trav_label -> Prop) :=
-  dom_rel (iord G sc ;; <|tc|>) ⊆₁ tc.
+(* Notation "'Rel'" := (is_rel lab). *)
+Notation "'Rel'" := (fun x => is_true (is_rel lab x)).
+
   
 Definition iiord_step (tl : trav_label) : relation (trav_label -> Prop) :=
-  restr_rel iord_coherent
+  restr_rel (iord_coherent G sc)
             (<|fun tc => set_compl tc tl|> ;;
              (fun tc tc' => tc' ≡₁ tc ∪₁ eq tl)).
   
@@ -115,14 +257,188 @@ Definition isim_clos_step (tll : list trav_label)
 Definition sim_clos_step :=
   restr_rel sim_coherent 
             (fun tc tc' => exists tll, isim_clos_step tll tc tc').
+
+
+
+Section IssueClosure.
+  Variable (tc: trav_label -> Prop). 
+  Variable (e: actid).
+  Let lbl := (ta_issue, e). 
+  Let tc' := tc ∪₁ eq lbl. 
+  Let stc := sim_clos tc.
+  Let stc' := sim_clos tc'. 
   
+  Hypothesis (ICOH: iord_coherent G sc tc). 
+  Hypothesis (ICOH': iord_coherent G sc tc').
+  Hypothesis (TCOH: tls_coherent G tc). 
+  Hypothesis (TCOH': tls_coherent G tc'). 
+  (* Hypothesis (TRAV_STEP : itrav_step G sc e tc tc').  *)
+  Hypothesis (NISS: ~ tc lbl).
+  (* Hypothesis (ISS: issuable G sc tc e). *)
+  
+  (* Let irel_crmw := I ∩₁ (is_rel lab) ∪₁ codom_rel (⦗C⦘ ⨾ rmw). *)
+  Lemma rel_clos_dist (tc1 tc2: trav_label -> Prop):
+    rel_clos (tc1 ∪₁ tc2) ≡₁ rel_clos tc1 ∪₁ rel_clos tc2. 
+  Proof. 
+    unfold rel_clos. rewrite !set_pair_alt. unfold tl_issued. basic_solver 10.
+  Qed. 
+    
+  Lemma rmw_clos_dist (tc1 tc2: trav_label -> Prop):
+    rmw_clos (tc1 ∪₁ tc2) ≡₁ rmw_clos tc1 ∪₁ rmw_clos tc2. 
+  Proof. 
+    unfold rmw_clos. rewrite !set_pair_alt. unfold tl_covered. basic_solver 10.
+  Qed. 
+
+  Lemma sim_clos_dist (tc1 tc2: trav_label -> Prop):
+    sim_clos (tc1 ∪₁ tc2) ≡₁ sim_clos tc1 ∪₁ sim_clos tc2. 
+  Proof. 
+    unfold sim_clos. rewrite rel_clos_dist, rmw_clos_dist. basic_solver. 
+  Qed. 
+
+  Global Add Parametric Morphism : sim_clos with signature
+      set_equiv ==> set_equiv as sim_clos_more.
+  Proof using.
+    unfold sim_clos. ins. unfold rmw_clos, rel_clos, tl_issued, tl_covered.
+    rewrite !set_pair_alt. rewrite H. basic_solver.
+  Qed.
+
+  Global Add Parametric Morphism : sim_clos_step with signature
+         set_equiv ==> set_equiv ==> iff as sim_clos_step_more.
+  Proof using. ins. apply set_extensionality in H, H0. by subst. Qed.
+
+  Global Add Parametric Morphism
+         {A: Type} (r: relation (A -> Prop)):
+    r with signature
+         @set_equiv A ==> @set_equiv A ==> iff as set_equiv_rel_more. 
+  Proof using. ins. apply set_extensionality in H, H0. by subst. Qed.
+
+  
+  Lemma trav_step_closures_isim_issue
+        WF
+        (* WFSC CONS COMP *)
+    :
+    (* same_trav_config {| *)
+    (*     covered := *)
+    (*     C *)
+    (*       ∪₁ (I ∩₁ (fun a : actid => is_rel lab a) ∪₁ codom_rel (⦗C⦘ ⨾ rmw)) \₁ C; *)
+    (*     issued := I ∪₁ codom_rel (⦗C⦘ ⨾ rmw) \₁ I *)
+    (*   |} (sim_trav_closure G tc) -> *)
+    (* same_trav_config {| *)
+    (*     covered := *)
+    (*     C *)
+    (*       ∪₁ ((I ∪₁ eq e) ∩₁ (fun a : actid => is_rel lab a) *)
+    (*                       ∪₁ codom_rel (⦗C⦘ ⨾ rmw)) \₁ C; *)
+    (*     issued := I ∪₁ eq e ∪₁ codom_rel (⦗C⦘ ⨾ rmw) \₁ (I ∪₁ eq e) *)
+    (*   |} (sim_trav_closure G tc') -> *)
+    sim_clos_step＊ stc stc'.
+  Proof using. 
+    rename e into w.
+    assert (W w) as Ww.
+    { replace w with (event lbl); auto. eapply (@tlsc_I_in_W _ tc'); eauto. 
+      subst tc'. basic_solver. }
+    assert (~ tc (mkTL ta_cover w)) as NCw.
+    { intros Cw. forward eapply (@tlsc_w_covered_issued _ _ tc) as WCI; eauto.
+      destruct NISS. specialize (WCI (mkTL ta_cover w)). specialize_full WCI.
+      { basic_solver. }
+      unfolder in WCI. desc. subst lbl. destruct y. simpl in *. subst.
+      red in WCI. unfolder in WCI. desc. simpl in *. congruence. }
+    
+  (*   rewrite set_inter_union_l, set_unionA. *)
+  (*   rewrite set_unionC with (s := eq w ∩₁ _), <- set_unionA. *)
+  (*   rewrite set_minus_union_l with (s' := eq w ∩₁ _). *)
+  (*   rewrite set_minus_disjoint with (s1 := eq w ∩₁ _); [| basic_solver]. *)
+  (*   rewrite <- set_minus_minus_l, set_unionA. *)
+  (*   rewrite <- set_union_strict with (s1 := eq w). *)
+
+    assert (rmw_clos (eq lbl) ≡₁ ∅) as NO_RMWC.
+    { apply set_subset_empty_r. unfold rmw_clos.
+      rewrite set_pair_alt. erewrite wf_rmwD; eauto. 
+      subst lbl. unfold tl_covered. type_solver. }
+
+    generalize (set_equiv_refl2 stc),  (set_equiv_refl2 stc').
+    unfold stc at 2, stc' at 2. unfold sim_clos, tc'.
+    rewrite rmw_clos_dist, rel_clos_dist. rewrite NO_RMWC, set_union_empty_r.
+    rewrite set_unionA with (s'' := _ ∪₁ _), set_unionC with (s := rmw_clos tc).
+    rewrite set_unionA with (s' := rel_clos _).
+
+    (***)
+    arewrite (rel_clos (eq lbl) ≡₁ (event ↓₁ Rel) ∩₁ eq (mkTL ta_cover w)).
+    { unfold rel_clos, tl_issued. rewrite set_pair_alt.
+      red. subst lbl. split; unfolder; ins; desc; destruct x; ins. 
+      { subst. vauto. }
+      inversion H0. subst. splits; vauto. }
+    (***)
+        
+    destruct (classic (codom_rel (⦗tl_covered tc⦘ ⨾ rmw) w)) as [CRMWw | NCRMWw].
+    { apply set_subset_single_l in CRMWw. 
+      rewrite set_union_absorb_l with (s := _ ∩₁ _).
+      2: { unfold rel_clos, rmw_clos, tl_issued. rewrite !set_pair_alt.
+           rewrite <- CRMWw. basic_solver. }
+      rewrite set_unionA with (s' := eq _).
+      rewrite set_union_absorb_l with (s := eq _).
+      2: { apply set_subset_union_r. right. unfold rmw_clos.
+           rewrite set_pair_alt. rewrite <- CRMWw. basic_solver. }
+      intros -> ->. rewrite set_unionC with (s := rel_clos _), <- set_unionA.
+      apply rt_refl. }
+          
+    destruct (classic (Rel w)) as [RELw | NRELw].
+    2: { erewrite (proj1 (set_disjointE _ _)), set_union_empty_l; [|basic_solver].
+         (* rewrite (proj1 (set_disjointE (eq w) Rel)); [| basic_solver]. *)
+         (* rewrite set_union_empty_r. *)
+      
+         foobar. 
+         fold irel_crmw.
+         rewrite set_unionC with (s := eq w), <- set_unionA.
+         intros <- <-.
+         apply rt_step. apply rlx_write_promise_step; auto.
+         { simpl. intros [? | [?]]; basic_solver. }
+         simpl. apply itrav_step_mon_ext_issue.
+         { by fold tc tc'. }
+         simpl. apply set_disjoint_eq_r. intros [? | [?]]; basic_solver. }
+    
+  (*   rewrite set_inter_absorb_r with (s := eq w); [| basic_solver]. *)
+  (*   fold irel_crmw. *)
+    
+  (*   rewrite set_unionC with (s := eq w), <- !set_unionA. *)
+  (*   intros STC STC'. rewrite <- STC, <- STC'. *)
+  (*   apply rt_step. apply rel_write_step; auto. *)
+  (*   { intros [r RMW]. apply NCRMWw. exists r. apply seq_eqv_l. split; auto. *)
+  (*     cdes ISS. apply proj1, proj2 in ISS0. red in ISS0. apply ISS0. *)
+  (*     red. exists w. apply seq_eqv_r. split; auto. *)
+  (*     red. repeat left. apply seq_eqv_r. split; [| basic_solver]. *)
+  (*     by apply rmw_in_sb. } *)
+  (*   { simpl. intros [? | [?]]; basic_solver. } *)
+  (*   { simpl. apply itrav_step_mon_ext_issue. *)
+  (*     { by fold tc tc'. } *)
+  (*     simpl. apply set_disjoint_eq_r. intros [? | [?]]; basic_solver. } *)
+    
+  (*   simpl. red. left. splits. *)
+  (*   3, 4: simpl; basic_solver. *)
+  (*   { simpl. unfold irel_crmw. intros [? | IC]; [by auto| ]. *)
+  (*     red in IC. desc. destruct IC as [IC | IC]; auto. *)
+  (*     destruct NISS. apply IC. } *)
+  (*   simpl. apply coverable_add_eq_iff; auto. *)
+  (*   simpl. apply covered_in_coverable; [| simpl; basic_solver]. *)
+  (*   rewrite STC'. apply stc_coherent; auto. *)
+  (* Qed. *)
+  Admitted. 
+  
+End IssueClosure.
+
 Lemma iord_step_implies_sim_clos_step :
   iord_step ⊆ sim_clos ↓ sim_clos_step^*.
 Proof using.
-  unfolder; intros x y STEP.
-  red in STEP. desf.
+  unfolder; intros tc tc' STEP.
+  red in STEP. destruct STEP as [[a e] STEP]. 
+  do 2 red in STEP. desc. apply seq_eqv_l in STEP. desc.
+
+  destruct a.
+  2: { replace tc' with (tc ∪₁ eq (ta_issue, e)) by admit. 
+       apply trav_step_closures_isim_issue; auto. }
+  
 
   (* use trav_step_closures_isim from SimTravClosure.v  *)
 Admitted.
+  
 
 End TravOrderConfig.
